README.md
@@ -1,1 +1,6 @@
 # loom2
+
+TODOs:
+  1. Change `wp_pure` to `⊑`
+  2. Change epost to List of types
+  3. ...
